add measure for graph marking algorithm

schorr-waite/GraphMark.thy
@@ -5,26 +5,40 @@ begin
 install_C_file "graph_mark.c"
 autocorres [heap_abs_syntax] "graph_mark.c"
 
-definition f_star :: "('a \<Rightarrow> 'a set) \<Rightarrow> ('a \<Rightarrow> 'a set)" where
-  "f_star f p = rtrancl { p. snd p \<in> f (fst p) } `` { p }"
+definition reach :: "('a \<Rightarrow> 'a set) \<Rightarrow> 'a set \<Rightarrow> 'a set" where
+  "reach f roots = rtrancl { p. snd p \<in> f (fst p) } `` roots"
 
 context graph_mark begin
 
-definition ok :: "node_C ptr \<Rightarrow> lifted_globals \<Rightarrow> bool" where
+type_synonym state_pred = "lifted_globals \<Rightarrow> bool"
+
+definition ok :: "node_C ptr \<Rightarrow> state_pred" where
   "ok p s \<equiv> p \<noteq> NULL \<and> is_valid_node_C s p"
 
-definition reach :: "lifted_globals \<Rightarrow> node_C ptr \<Rightarrow> node_C ptr set" where
-  "reach s \<equiv> f_star (\<lambda> p. { s[p]\<rightarrow>left, s[p]\<rightarrow>right })"
+definition out :: "lifted_globals \<Rightarrow> node_C ptr \<Rightarrow> node_C ptr set" where
+  "out s p \<equiv> { s[p]\<rightarrow>left, s[p]\<rightarrow>right }"
 
 definition mark :: "bool \<Rightarrow> node_C \<Rightarrow> node_C" where
   "mark c node \<equiv> if c then node \<lparr> mark_C := 3 \<rparr> else node"
 
-lemma graph_mark'_correct:
-  "\<lbrace> \<lambda> s. s = i \<and> (\<forall> p \<in> reach s root. ok p s \<and> s[p]\<rightarrow>mark = 0) \<rbrace>
-    graph_mark' root
-   \<lbrace> \<lambda> _ s. s = heap_node_C_update (\<lambda> h p. mark (p \<in> reach s root) (h p)) i \<rbrace>!"
+definition mark_pre :: "state_pred \<Rightarrow> node_C ptr \<Rightarrow> state_pred" where
+  "mark_pre P root \<equiv> \<lambda> s. let R = reach (out s) {root} in
+    (\<forall> p \<in> R. ok p s \<and> s[p]\<rightarrow>mark = 0) \<and> P (heap_node_C_update (\<lambda> h p. mark (p \<in> R) (h p)) s)"
+
+primrec mark_invariant :: "state_pred \<Rightarrow> node_C ptr \<Rightarrow> node_C ptr \<times> node_C ptr \<Rightarrow> state_pred" where
+  "mark_invariant P root (p,q) s = True"
+
+primrec roots :: "node_C ptr \<times> node_C ptr \<Rightarrow> node_C ptr set" where
+  "roots (p,q) = { r \<in> {p,q}. r \<noteq> NULL }"
+
+primrec mark_measure :: "(node_C ptr \<times> node_C ptr) \<times> lifted_globals \<Rightarrow> nat" where
+  "mark_measure (r,s) = setsum (\<lambda> p. 3 - unat s[p]\<rightarrow>mark) (reach (out s) (roots r))"
+
+lemma graph_mark'_correct: "\<lbrace> mark_pre P root \<rbrace> graph_mark' root \<lbrace> \<lambda> _. P \<rbrace>!"
   unfolding
-    graph_mark'_def
+    graph_mark'_def mark_pre_def
+    whileLoop_add_inv[where I="mark_invariant P root" and M="mark_measure"]
+  apply (wp; clarsimp)
   sorry
 
 end
